

$$\#5. (12.23) \quad \| \tau_h \|_h^2 \leq 3 \left(\| f \|_h^2 + \| f \|_{L^2(0,1)}^2 \right).$$

$$R_+(x_j + h) = \int_{x_j}^{x_j + h} (u'''(\tau) - u'''(x_j)) \frac{(x_j + h - \tau)^2}{2} d\tau.$$

$$R_+(x_j - h) = - \int_{x_j - h}^{x_j} (u'''(\tau) - u'''(x_j)) \frac{(x_j - h - \tau)^2}{2} d\tau$$

$$\tau_h(x_j) = \frac{1}{h^2} (R_+(x_j + h) + R_+(x_j - h)) \quad (12.21).$$

$$\rightarrow R_+(x_j + h) = \underbrace{\int_{x_j}^{x_j + h} u'''(\tau) \frac{(x_j + h - \tau)^2}{2} d\tau}_{\textcircled{1}} - u'''(x_j) \underbrace{\int_{x_j}^{x_j + h} \frac{(x_j + h - \tau)^2}{2} d\tau}_{\textcircled{2}}.$$

$$\textcircled{1} \text{ Let } du^* = u'''(\tau) \Rightarrow u^* = u''(\tau).$$

$$v = \frac{(x_j + h - \tau)^2}{2} \Rightarrow dv = x_j + h - \tau$$

$$\Rightarrow \textcircled{1} = \frac{h^2}{2} u'' \Big|_{x_j}^{x_j + h} - \int_{x_j}^{x_j + h} u''(x_j + h - \tau) d\tau.$$

$$\textcircled{2} = -\frac{h^2}{2} u'''(x_j)$$

$$\Rightarrow R_+(x_j + h) = -\frac{h^2}{2} u''(x_j) - \frac{h^3}{6} u'''(x_j) + \int_{x_j}^{x_j + h} u''(x_j + h - \tau) d\tau$$

$$\text{Similarly, } R_+(x_j - h) = \frac{h^2}{2} u''(x_j) - \frac{h^3}{6} u'''(x_j) + \int_{x_j - h}^{x_j} u''(x_j - h - \tau) d\tau.$$

$$\Rightarrow \tau_h(x_j) = -u''(x_j) + \frac{1}{h^2} \left(\int_{x_j}^{x_j + h} u''(\tau) (x_j + h - \tau) d\tau - \int_{x_j - h}^{x_j} u''(\tau) (x_j - h - \tau) d\tau \right)$$

On noted that.

$$(a+b+c)^2 \leq 3(a^2+b^2+c^2), \text{ we have.}$$

$$\frac{1}{3} \tau_n^2(x_j) = u''(x_j)^2 + \underbrace{\frac{1}{h^4} \left(\int_{x_j}^{x_j+h} u''(t)(x_j+h-t) dt \right)^2}_{(A)} + \underbrace{\frac{1}{h^4} \left(\int_{x_j-h}^{x_j} u''(t)(x_j-h-t) dt \right)^2}_{(B)}$$

(A) by Cauchy-Schwarz.

$$\begin{aligned} (A) &= \frac{1}{h^4} \int_{x_j}^{x_j+h} u''(t)^2 dt \int_{x_j}^{x_j+h} (x_j+h-t)^2 dt \\ &\leq \frac{1}{3h} \int_{x_j}^{x_j+h} u''(t)^2 dt \quad \text{since } |x_j+h-t| \leq h \text{ for } t \in [x_j, x_j+h]. \end{aligned}$$

Similarly.

$$(B) \leq \frac{1}{3h} \int_{x_j-h}^{x_j} u''(t)^2 dt.$$

$$\Rightarrow \sum_{j=1}^{n-1} \tau_h(x_j)^2 \leq 3 \sum_{j=1}^{n-1} u''(x_j)^2 + \frac{1}{h} \sum_{j=1}^{n-1} \int_{x_j-h}^{x_j} u''(t)^2 dt + \frac{1}{h} \sum_{j=1}^{n-1} \int_{x_j}^{x_j+h} u''(t)^2 dt.$$

$$\Rightarrow \| \tau_n \|_h^2 \leq h \sum_{j=1}^{n-1} \tau_h(x_j)^2 \leq 3h \sum_{j=1}^{n-1} u''(x_j)^2 + \sum_{j=1}^{n-1} \int_{x_j-h}^{x_j} u''(t)^2 dt + \sum_{j=1}^{n-1} \int_{x_j}^{x_j+h} u''(t)^2 dt.$$

$$\leq 3 \| u'' \|_h^2 + 3 \int_{x_0}^{x_n} u''(t)^2 dt.$$

$$= 3 \| u'' \|_h^2 + 3 \| u'' \|_{L^2(0,1)}^2.$$

$$= 3 \| f \|_h^2 + 3 \| f \|_{L^2(0,1)}^2 \quad (-u'' = f) \quad \square.$$

#7. (12.25) $w_h = T_h g$, $w_h = \sum_{k=1}^{n-1} g(x_k) G^k$

$w_k(x_j) = \sum_{k=1}^{n-1} g(x_k) G^k(x_j)$, given $g(x_k) = 1$, and $G^k(x_j) = \frac{1}{h} G(x_j, x_k)$ #6.

$$T_h g(x_j) = h \left(\sum_{k=1}^{j-1} x_k (1-x_j) + \sum_{k=j+1}^{n-1} x_j (1-x_k) \right)$$

$$= h \left((1-x_j) \sum_{k=1}^{j-1} x_k + x_j \sum_{k=j+1}^{n-1} (1-x_k) \right) \quad (*)$$

On uniform grid, $x_k = kh$,

$$(*) = h \left((1-jh) \frac{(1+j)jh}{(1-jh)(1+jh)} + jh \left((n-j-1) - h \frac{(n-j-1)(n+j)}{2} \right) \right)$$

$$= jh \cdot \frac{1}{2} \left(h - jh^2 + jh - j^2 h^2 + 2nh - 2jh - 2h - n^2 h^2 + j^2 h^2 + nh^2 + jh^2 \right)$$

$$= \frac{x_j}{2} \left(2nh - jh - h - n^2 h^2 + nh^2 \right) = \frac{x_j}{2} \cdot h \cdot (n-j) = \frac{x_j}{2} (1-x_j) \quad (\text{take } h = \frac{1}{n})$$

#8 Prove Young's inequality $ab \leq \varepsilon a^2 + \frac{1}{4\varepsilon} b^2$, $\forall a, b \in \mathbb{R}$, $\forall \varepsilon > 0$. (12.40)

Consider $0 \leq \left(\sqrt{\varepsilon} a - \frac{b}{2\sqrt{\varepsilon}} \right)^2 = \varepsilon a^2 - ab + \frac{1}{4\varepsilon} b^2$

$$\Rightarrow ab \leq \varepsilon a^2 + \frac{1}{4\varepsilon} b^2$$

#9 Show that $\|v_h\|_h \leq \|v_h\|_{h,\infty}$ $\forall v_h \in V_h$.

$$\|v_h\|_h^2 = h \sum_{j=1}^{n-1} v_h(x_j)^2, \quad \|v_h\|_{h,\infty}^2 = \max_{1 \leq j \leq n-1} v_h^2$$

By def, $(v_h(x_j))^2 \leq (\|v_h\|_{h,\infty})^2$ for all j .

$$\Rightarrow h \sum_{j=1}^{n-1} (v_h(x_j))^2 \leq h \sum_{j=1}^{n-1} (\|v_h\|_{h,\infty})^2 = h \cdot (n-1) \|v_h\|_{h,\infty}^2 \leq \|v_h\|_{h,\infty}^2$$

$$\Rightarrow \|v_h\|_h^2 \leq \|v_h\|_{h,\infty}^2 \Rightarrow \|v_h\|_h \leq \|v_h\|_{h,\infty} \quad \square$$

11 the fourth-order $L_n(x) = -u^{(iv)}(x)$ from centered finite difference.

$$L_n w(x_j) = - \frac{w_{j+1} - 2w_j + w_{j-1}}{h^2}$$

$$x_{j+1} = - \frac{w_{j+2} - 2w_{j+1} + w_j}{h^2}$$

$$x_{j-1} = - \frac{w_j - 2w_{j-1} + w_{j-2}}{h^2}$$

$$(L_n w)^2(x_j) = - \frac{L_n w_{j+1} - 2L_n w_j + L_n w_{j-1}}{h^2}$$

$$= - \frac{1}{h^2} \cdot \left(- \frac{1}{h^2} \right) \left(\underbrace{w_{j+2} - 2w_{j+1} + w_j}_{\Delta} - 2 \underbrace{w_{j+1} - 2w_j + w_{j-1}}_{\Delta} + \underbrace{w_j - 2w_{j-1} + w_{j-2}}_{\Delta} \right)$$

$$= \frac{1}{h^4} \left(w_{j+2} - 4w_{j+1} + 6w_j - 4w_{j-1} + w_{j-2} \right)$$

$$\Rightarrow L_n(x) = -u^{(iv)}(x) = -L_n^2 w(x_j) = \frac{-1}{h^4} (w_{j+2} - 4w_{j+1} + 6w_j - 4w_{j-1} + w_{j-2})$$